examples/sbf/verif.v
@@ -390,72 +390,77 @@ Proof.
   unfold Row_tbl_bloom_fundef.
 
   hoare_func_table.
-  { apply hoare_extern_match_list_intro. }
   simpl Tofino.extern_matches.
   econstructor.
   (* INSERT case *)
-  { reflexivity. }
-  { intros.
-    step_call Row_insert_body.
-    3 : { entailer. }
-    { auto. }
-    { auto. }
-    apply ret_implies_refl.
-  }
-  { constructor. }
-  { intros.
-    assert (op = INSERT). {
-      repeat destruct x0 as [? | x0]; subst; try solve [inv H].
-      auto.
-      destruct x0.
+  { econstructor.
+    { reflexivity. }
+    { intros.
+      step_call Row_insert_body.
+      3 : { entailer. }
+      { auto. }
+      { auto. }
+      apply ret_implies_refl.
     }
-    subst.
-    apply arg_ret_implies_post_ex. eexists.
-    entailer.
+    { constructor. }
+    { intros.
+      assert (op = INSERT). {
+        repeat destruct x0 as [? | x0]; subst; try solve [inv H].
+        auto.
+        destruct x0.
+      }
+      subst.
+      apply arg_ret_implies_post_ex. eexists.
+      entailer.
+    }
   }
   econstructor.
   (* QUERY case *)
-  { reflexivity. }
-  { intros.
-    step_call Row_query_body.
-    3 : { entailer. }
-    { auto. }
-    { auto. }
-    apply ret_implies_refl.
-  }
-  { constructor. }
-  { intros.
-    assert (op = QUERY). {
-      repeat destruct x0 as [? | x0]; subst; try solve [inv H0].
-      auto.
-      destruct x0.
+  { econstructor.
+    { reflexivity. }
+    { intros.
+      step_call Row_query_body.
+      3 : { entailer. }
+      { auto. }
+      { auto. }
+      apply ret_implies_refl.
     }
-    subst.
-    apply arg_ret_implies_post_ex. eexists.
-    entailer.
-    destruct (row_query r i);
-      apply sval_refine_refl.
+    { constructor. }
+    { intros.
+      assert (op = QUERY). {
+        repeat destruct x0 as [? | x0]; subst; try solve [inv H0].
+        auto.
+        destruct x0.
+      }
+      subst.
+      apply arg_ret_implies_post_ex. eexists.
+      entailer.
+      destruct (row_query r i);
+        apply sval_refine_refl.
+    }
   }
   econstructor.
   (* CLEAR case *)
-  { reflexivity. }
-  { intros.
-    step_call Row_clear_body.
-    3 : { entailer. }
-    { auto. }
-    { auto. }
-    apply ret_implies_refl.
-  }
-  { constructor. }
-  { intros.
-    assert (op = CLEAR). {
-      repeat destruct x0 as [? | x0]; subst; try solve [inv H1].
-      auto.
-      destruct x0.
+  { econstructor.
+    { reflexivity. }
+    { intros.
+      step_call Row_clear_body.
+      3 : { entailer. }
+      { auto. }
+      { auto. }
+      apply ret_implies_refl.
     }
-    subst.
-    apply arg_ret_implies_post_ex. eexists.
-    entailer.
+    { constructor. }
+    { intros.
+      assert (op = CLEAR). {
+        repeat destruct x0 as [? | x0]; subst; try solve [inv H1].
+        auto.
+        destruct x0.
+      }
+      subst.
+      apply arg_ret_implies_post_ex. eexists.
+      entailer.
+    }
   }
   (* NOOP case *)
   (* We cannot prove the NOOP case with the current spec. *)
@@ -476,323 +481,6 @@ Proof.
   step_call Row_tbl_bloom_body.
   4 : entailer.
   1-3 : auto.
-  Intros _.
-  step.
-  entailer.
-Qed.
-
-Definition Row_noop_case_spec : func_spec :=
-  WITH (* p *),
-    PATH p
-    MOD None [p]
-    WITH (r : row) (i : Z)
-      (_ : Zlength r = num_cells)
-      (_ : 0 <= i < Zlength r),
-      PRE
-        (ARG [eval_val_to_sval (ValBaseBit (P4Arith.to_lbool 8%N NOOP));
-              eval_val_to_sval (ValBaseBit (P4Arith.to_lbool 18%N i))]
-        (MEM []
-        (EXT [row_repr p r])))
-      POST
-        (ARG_RET [ValBaseBit (Zrepeat None 8)] ValBaseNull
-        (MEM []
-        (EXT [row_repr p r]))).
-
-Definition Row_tbl_bloom_noop_spec : func_spec :=
-  WITH (* p *),
-    PATH p
-    MOD (Some [["rw"]]) [p]
-    WITH (r : row) (i : Z)
-      (_ : Zlength r = num_cells)
-      (_ : 0 <= i < Zlength r),
-      PRE
-        (ARG []
-        (MEM [(["api"], eval_val_to_sval (ValBaseBit (P4Arith.to_lbool 8%N NOOP)));
-              (["index"], eval_val_to_sval (ValBaseBit (P4Arith.to_lbool 18%N i)));
-              (["rw"], ValBaseBit (Zrepeat None 8))]
-        (EXT [row_repr p r])))
-      POST
-        (EX retv,
-        (ARG_RET [] retv
-        (MEM [(["rw"], ValBaseBit (Zrepeat None 8))]
-        (EXT [row_repr p r]))))%arg_ret_assr.
-
-Lemma Row_tbl_bloom_noop_body :
-  func_sound ge Row_tbl_bloom_fundef nil Row_tbl_bloom_noop_spec.
-Proof.
-  split. 2 : {
-    solve_modifies.
-  }
-  intros_fsh_bind.
-  red.
-  unfold Row_tbl_bloom_fundef.
-  hoare_func_table.
-  { instantiate (1 := [(true, mk_action_ref "NoAction" [])]).
-    constructor.
-  }
-  econstructor.
-  (* NOOP case *)
-  { reflexivity. }
-  { intros.
-    step_call NoAction_body.
-    { entailer. }
-    apply ret_implies_refl.
-  }
-  { constructor. }
-  { intros.
-    apply arg_ret_implies_post_ex. eexists.
-    entailer.
-  }
-  intros H; inv H.
-Qed.
-
-Lemma Row_noop_case_body :
-  func_sound ge Row_fundef nil Row_noop_case_spec.
-Proof.
-  start_function.
-  step.
-  step_call Row_tbl_bloom_noop_body.
-  3 : entailer.
-  1-2 : auto.
-  Intros _.
-  step.
-  entailer.
-Qed.
-
-Definition Row_insert_case_spec : func_spec :=
-  WITH (* p *),
-    PATH p
-    MOD None [p]
-    WITH (r : row) (i : Z)
-      (_ : Zlength r = num_cells)
-      (_ : 0 <= i < Zlength r),
-      PRE
-        (ARG [eval_val_to_sval (ValBaseBit (P4Arith.to_lbool 8%N INSERT));
-              eval_val_to_sval (ValBaseBit (P4Arith.to_lbool 18%N i))]
-        (MEM []
-        (EXT [row_repr p r])))
-      POST
-        (ARG_RET [eval_val_to_sval (ValBaseBit (P4Arith.to_lbool 8 1))] ValBaseNull
-        (MEM []
-        (EXT [row_repr p (row_insert r i)]))).
-
-Definition Row_tbl_bloom_insert_spec : func_spec :=
-  WITH (* p *),
-    PATH p
-    MOD (Some [["rw"]]) [p]
-    WITH (r : row) (i : Z)
-      (_ : Zlength r = num_cells)
-      (_ : 0 <= i < Zlength r),
-      PRE
-        (ARG []
-        (MEM [(["api"], eval_val_to_sval (ValBaseBit (P4Arith.to_lbool 8%N INSERT)));
-              (["index"], eval_val_to_sval (ValBaseBit (P4Arith.to_lbool 18%N i)))]
-        (EXT [row_repr p r])))
-      POST
-        (EX retv,
-        (ARG_RET [] retv
-        (MEM [(["rw"], eval_val_to_sval (ValBaseBit (P4Arith.to_lbool 8 1)))]
-        (EXT [row_repr p (row_insert r i)]))))%arg_ret_assr.
-
-Lemma Row_tbl_bloom_insert_body :
-  func_sound ge Row_tbl_bloom_fundef nil Row_tbl_bloom_insert_spec.
-Proof.
-  split. 2 : {
-    solve_modifies.
-  }
-  intros_fsh_bind.
-  red.
-  unfold Row_tbl_bloom_fundef.
-  hoare_func_table.
-  { instantiate (1 := [(true, mk_action_ref "act_insert" [])]).
-    constructor.
-  }
-  econstructor.
-  (* INSERT case *)
-  { reflexivity. }
-  { intros.
-    step_call Row_insert_body.
-    3 : { entailer. }
-    { auto. }
-    { auto. }
-    apply ret_implies_refl.
-  }
-  { constructor. }
-  { intros.
-    apply arg_ret_implies_post_ex. eexists.
-    entailer.
-  }
-  intros H; inv H.
-Qed.
-
-Lemma Row_insert_case_body :
-  func_sound ge Row_fundef nil Row_insert_case_spec.
-Proof.
-  start_function.
-  step.
-  step_call Row_tbl_bloom_insert_body.
-  3 : entailer.
-  1-2 : auto.
-  Intros _.
-  step.
-  entailer.
-Qed.
-
-Definition Row_query_case_spec : func_spec :=
-  WITH (* p *),
-    PATH p
-    MOD None [p]
-    WITH (r : row) (i : Z)
-      (_ : Zlength r = num_cells)
-      (_ : 0 <= i < Zlength r),
-      PRE
-        (ARG [eval_val_to_sval (ValBaseBit (P4Arith.to_lbool 8%N QUERY));
-              eval_val_to_sval (ValBaseBit (P4Arith.to_lbool 18%N i))]
-        (MEM []
-        (EXT [row_repr p r])))
-      POST
-        (ARG_RET [eval_val_to_sval (ValBaseBit (P4Arith.to_lbool 8 (Z.b2z (row_query r i))))] ValBaseNull
-        (MEM []
-        (EXT [row_repr p r]))).
-
-Definition Row_tbl_bloom_query_spec : func_spec :=
-  WITH (* p *),
-    PATH p
-    MOD (Some [["rw"]]) [p]
-    WITH (r : row) (i : Z)
-      (_ : Zlength r = num_cells)
-      (_ : 0 <= i < Zlength r),
-      PRE
-        (ARG []
-        (MEM [(["api"], eval_val_to_sval (ValBaseBit (P4Arith.to_lbool 8%N QUERY)));
-              (["index"], eval_val_to_sval (ValBaseBit (P4Arith.to_lbool 18%N i)))]
-        (EXT [row_repr p r])))
-      POST
-        (EX retv,
-        (ARG_RET [] retv
-        (MEM [(["rw"], eval_val_to_sval (ValBaseBit (P4Arith.to_lbool 8 (Z.b2z (row_query r i)))))]
-        (EXT [row_repr p r]))))%arg_ret_assr.
-
-Lemma Row_tbl_bloom_query_body :
-  func_sound ge Row_tbl_bloom_fundef nil Row_tbl_bloom_query_spec.
-Proof.
-  split. 2 : {
-    solve_modifies.
-  }
-  intros_fsh_bind.
-  red.
-  unfold Row_tbl_bloom_fundef.
-  hoare_func_table.
-  { instantiate (1 := [(true, mk_action_ref "act_query" [])]).
-    constructor.
-  }
-  econstructor.
-  (* QUERY case *)
-  { reflexivity. }
-  { intros.
-    step_call Row_query_body.
-    3 : { entailer. }
-    { auto. }
-    { auto. }
-    apply ret_implies_refl.
-  }
-  { constructor. }
-  { intros.
-    apply arg_ret_implies_post_ex. eexists.
-    entailer.
-    destruct (row_query r i);
-      apply sval_refine_refl.
-  }
-  intros H; inv H.
-Qed.
-
-Lemma Row_query_case_body :
-  func_sound ge Row_fundef nil Row_query_case_spec.
-Proof.
-  start_function.
-  step.
-  step_call Row_tbl_bloom_query_body.
-  3 : entailer.
-  1-2 : auto.
-  Intros _.
-  step.
-  entailer.
-Qed.
-
-Definition Row_clear_case_spec : func_spec :=
-  WITH (* p *),
-    PATH p
-    MOD None [p]
-    WITH (r : row) (i : Z)
-      (_ : Zlength r = num_cells)
-      (_ : 0 <= i < Zlength r),
-      PRE
-        (ARG [eval_val_to_sval (ValBaseBit (P4Arith.to_lbool 8%N CLEAR));
-              eval_val_to_sval (ValBaseBit (P4Arith.to_lbool 18%N i))]
-        (MEM []
-        (EXT [row_repr p r])))
-      POST
-        (ARG_RET [eval_val_to_sval (ValBaseBit (P4Arith.to_lbool 8 0))] ValBaseNull
-        (MEM []
-        (EXT [row_repr p (row_clear r i)]))).
-
-Definition Row_tbl_bloom_clear_spec : func_spec :=
-  WITH (* p *),
-    PATH p
-    MOD (Some [["rw"]]) [p]
-    WITH (r : row) (i : Z)
-      (_ : Zlength r = num_cells)
-      (_ : 0 <= i < Zlength r),
-      PRE
-        (ARG []
-        (MEM [(["api"], eval_val_to_sval (ValBaseBit (P4Arith.to_lbool 8%N CLEAR)));
-              (["index"], eval_val_to_sval (ValBaseBit (P4Arith.to_lbool 18%N i)))]
-        (EXT [row_repr p r])))
-      POST
-        (EX retv,
-        (ARG_RET [] retv
-        (MEM [(["rw"], eval_val_to_sval (ValBaseBit (P4Arith.to_lbool 8 0)))]
-        (EXT [row_repr p (row_clear r i)]))))%arg_ret_assr.
-
-Lemma Row_tbl_bloom_clear_body :
-  func_sound ge Row_tbl_bloom_fundef nil Row_tbl_bloom_clear_spec.
-Proof.
-  split. 2 : {
-    solve_modifies.
-  }
-  intros_fsh_bind.
-  red.
-  unfold Row_tbl_bloom_fundef.
-  hoare_func_table.
-  { instantiate (1 := [(true, mk_action_ref "act_clear" [])]).
-    constructor.
-  }
-  econstructor.
-  (* CLEAR case *)
-  { reflexivity. }
-  { intros.
-    step_call Row_clear_body.
-    3 : { entailer. }
-    { auto. }
-    { auto. }
-    apply ret_implies_refl.
-  }
-  { constructor. }
-  { intros.
-    apply arg_ret_implies_post_ex. eexists.
-    entailer.
-  }
-  intros H; inv H.
-Qed.
-
-Lemma Row_clear_case_body :
-  func_sound ge Row_fundef nil Row_clear_case_spec.
-Proof.
-  start_function.
-  step.
-  step_call Row_tbl_bloom_clear_body.
-  3 : entailer.
-  1-2 : auto.
   Intros _.
   step.
   entailer.
